refactor: minor cosmetics

dev.v
@@ -2,198 +2,16 @@ From Coq Require Import Lia Relations.
 From mathcomp Require Import ssreflect ssrnat eqtype ssrbool ssrfun seq.
 From mathcomp Require Import finmap choice finfun fintype.
 From deriving Require Import deriving.
-From coqspec Require Import int.
-
-Ltac ssrnatify_rel :=
- match goal with
-  (* less or equal (also codes for strict comparison in ssrnat) *)
-  | H : is_true (leq _ _) |- _ => move/leP: H => H
-  | H : context [ is_true (leq ?a ?b)] |- _ =>
-     rewrite <- (rwP (@leP a b)) in H
-  | |- is_true (leq _ _) => apply/leP
-  | |- context [ is_true (leq ?a ?b)] => rewrite <- (rwP (@leP a b))
-  (* Boolean equality *)
-  | H : is_true (@eq_op _ _ _) |- _ => move/eqP: H => H
-  | |- is_true (@eq_op _ _ _) => apply/eqP
-  | H : context [ is_true (@eq_op _ _ _)] |- _ =>
-     rewrite <-  (rwP (@eqP _ _ _)) in H
-  | |- context [ is_true (@eq_op _ ?x ?y)] => rewrite <- (rwP (@eqP _ x y))
-  (* Negated boolean equality *)
-  | H : is_true (negb (@eq_op _  _ _)) |- _ => move/eqP: H => H
-  | |- is_true (negb (@eq_op _  _ _)) => apply/eqP
-  | H : context [ is_true (negb (@eq_op _ _ _))] |- _ =>
-     rewrite <-  (rwP (@eqP _ _ _)) in H
-  | |- context [ is_true (negb (@eq_op _ ?x ?y))] =>
-     rewrite <- (rwP (@eqP _ x y))
-  | H : (negb (@eq_op _  _ _)) = true |- _ => move/eqP: H => H
-  | |- (negb (@eq_op _  _ _)) = true => apply/eqP
-  | H : context [ (negb (@eq_op _ _ _)) = true ] |- _ =>
-     rewrite <-  (rwP (@eqP _ _ _)) in H
-  | |- context [ (negb (@eq_op _ ?x ?y)) = true ] =>
-     rewrite <- (rwP (@eqP _ x y))
-
-  | H : (leq _ _) = true |- _ => move/leP: H => H
-  | H : context [ (leq ?a ?b) = true] |- _ =>
-     rewrite <- (rwP (@leP a b)) in H
-  | |- (leq _ _) = true => apply/leP
-  | |- context [(leq ?a ?b) = true] => rewrite <- (rwP (@leP a b))
-  (* Boolean equality *)
-  | H : (@eq_op _ _ _) = true |- _ => move/eqP: H => H
-  | |- (@eq_op _ _ _) = true => apply/eqP
-  | H : context [(@eq_op _ _ _) = true] |- _ =>
-     rewrite <-  (rwP (@eqP _ _ _)) in H
-  | |- context [(@eq_op _ ?x ?y) = true] => rewrite <- (rwP (@eqP _ x y))
-
-  (* Negated lt *)
-  | H : is_true (negb (leq (S _) _)) |- _ => move: H; rewrite -leqNgt=> H
-  | H : context [ is_true (negb (leq (S _) _))] |- _ =>
-     rewrite -leqNgt in H
-  | |- is_true (negb (leq (S _) _)) => rewrite -leqNgt
-  | |- context [ is_true (negb (leq (S _) _))] => rewrite -leqNgt
-
-  (* Negated leq *)
-  | H : is_true (negb (leq _ _)) |- _ => move: H; rewrite -ltnNge=> H
-  | H : context [ is_true (negb (leq _ _))] |- _ =>
-     rewrite -ltnNge in H
-  | |- is_true (negb (leq _ _)) => rewrite -ltnNge
-  | |- context [ is_true (negb (leq _ _))] => rewrite -ltnNge
-
-   (* = flase *)
-  | H : (_ = false) |- _ => move/negbT: H => H
-  | |- (_ = false) => apply/negP
-  | H : context [ (?a = false)] |- _ =>
-     rewrite <-  (rwP (@negP a)) in H
-  | |- context [ ?a = false] =>
-     rewrite <- (rwP (@negP a))
-
- end.
-
-
-(* Converting ssrnat operation to their std lib analogues *)
-Ltac ssrnatify_op :=
- match goal with
-  (* subn -> minus *)
-  | H : context [subn _ _] |- _ => rewrite -!minusE in H
-  | |- context [subn _ _] => rewrite -!minusE
-  (* addn -> plus *)
-  | H : context [addn _ _] |- _ => rewrite -!plusE in H
-  | |- context [addn _ _] => rewrite -!plusE
-  (* muln -> mult *)
-  | H : context [muln _ _] |- _ => rewrite -!multE in H
-  | |- context [muln _ _] => rewrite -!multE
- end.
-
-(* Preparing a goal to be solved by lia by translating every formula *)
-(* in the context or the conclusion which expresses a constraint on *)
-(* some nat into the std lib, Prop, analogues *)
-Ltac ssrnatify :=
-  repeat progress ssrnatify_rel;
-  repeat progress ssrnatify_op.
-
-(* Preprocessing + lia *)
-Ltac slia := try (move=> * //=); do [ ssrnatify; lia | exfalso; ssrnatify; lia].
-
+From coqspec Require Import int utilities substitution.
 
 Set Implicit Arguments.
 Unset Printing Implicit Defensive.
-
-Inductive Restr := 
-  | Neq of Arg & Arg
-  | NCONS of Arg.
-
-Definition restr_indDef := [indDef for Restr_rect].
-Canonical restr_indType := IndType Restr restr_indDef.
-
-Definition restr_eqMixin := [derive eqMixin for Restr].
-Canonical restr_eqType := Eval hnf in EqType Restr restr_eqMixin.
-
-Definition restr_choiceMixin := [derive choiceMixin for Restr].
-Canonical restr_choiceType := Eval hnf in ChoiceType Restr restr_choiceMixin.
 
 Definition br_indDef := [indDef for Branch_rect].
 Canonical br_indType := IndType Branch br_indDef.
 
 Definition br_eqMixin := [derive eqMixin for Branch].
 Canonical br_eqType := Eval hnf in EqType Branch br_eqMixin.
-
-Notation "e1 '≠' e2" := (Neq e1 e2) (at level 10).
-
-Definition Cenv := (Env * seq Restr)%type.
-
-Inductive Bind :=
-  | isEQ of Arg & Arg
-  | isCONS of Arg.
-
-Definition contr  (b : Bind) (r : Restr) := 
-  match r, b with
-  | v ≠ u, isEQ v' u' => ((v, u) == (v', u')) || ((u, v) == (v', u'))
-  | NCONS v, isCONS u => v == u
-  | _, _              => false
-  end.
-
-Definition is_arg (e : Exp) := 
-  if e is Exp_Arg _ then true else false.
-
-Definition is_cons (e : Exp) := 
-  if e is CONS _ _ then true else false.
-
-
-Definition ncontr_neq env r1 r2 := 
-    is_arg (r1 /s/ env) ->
-    is_arg (r2 /s/ env) ->
-    r1 /s/ env <> r2 /s/ env.
-
-Definition ncontr_ncons env r := 
-  ~~ is_cons (r /s/ env).
-
-
-Definition ncontr_env (env : Env) (rs : seq Restr) := 
-  (forall r1 r2, r1 ≠ r2 \in rs -> ncontr_neq env r1 r2) /\
-  (forall r, NCONS r \in rs -> ncontr_ncons env r).
-
-
-Definition contradict r b : bool :=
-  has (contr b) r .
-
-Definition delete_restr (v : Var) := 
-  filter (fun r => match r with 
-                   | (r1 ≠ r2) => (r1 != v) && (r2 != v)
-                   | NCONS r => r != v
-                  end).
-
-Definition cas  (v u : Arg) (r : Restr) := 
-  if r is x ≠ y then 
-    (if x == v then u else x) ≠ (if y == v then u else y)
-  else r.
-
-
-Definition rsubst (r : seq Restr) (b : Bind) : seq Restr := 
-  match b with 
-  | isEQ u v => map (cas u v) r
-  | isCONS _ => r
-  end.
-
-Definition of_Bind b : Env := 
-  match b with 
-  | isEQ (Arg_Var u) v => [fsfun emsub with u |-> Exp_Arg v]
-  | _                  => emsub
-  end.
-
-Coercion of_Bind : Bind >-> Env.
-
-Definition b2r b : Restr := 
-  match b with
-  | isEQ u v => u ≠ v
-  | isCONS u => NCONS u
-  end.
-Coercion b2r : Bind >-> Restr.
-
-Definition csubst (c : Cenv) (e : Bind) := 
-  let: (ce, r) := c in
-  (comp ce e, rsubst r e).
-
-Definition restr (c : Cenv) (b : Bind) := 
-  let: (e, r) := c in (e, b2r b :: r).
 
 Inductive CBranch := 
   | CTRUE  of Cenv
@@ -235,21 +53,7 @@ Definition dev_cntr (c : Cntr) (ce : Cenv) : CBranch :=
 
 Section Spec.
 
-Variable p : Programm.
-
-Definition max_set (f : seq Var) : Var :=
-  foldr maxn 0 f.
-
-Fixpoint VTree (t : Tree) : {fset Var} :=
-  match t with
-  | RET e        => FVExp e
-  | LET v x t    => v |` (FVExp x `|` VTree t)
-  | COND c t1 t2 => FVCntr c `|` VTree t1 `|` VTree t2
-  | HT v u x t   => [fset v; u; x] `|`  (VTree t)
-  | CALL f xs    => seq_fset tt xs
-  end.
-
-Definition maxvar (t : Tree) : Var := max_set (VTree t).
+Variable p : Prog.
 
 Fixpoint dev (f : Var -> Tree -> Cenv -> Tree)
   (k : Var) (t : Tree) (e : Cenv) : Tree :=
@@ -269,7 +73,7 @@ Fixpoint dev (f : Var -> Tree -> Cenv -> Tree)
             v |-> Exp_Arg (k.+1 : Var),
             u |-> Exp_Arg (k.+2 : Var)], rs)
       ) 
-    | _ => RET '0
+    | _ => RET ERROR
     end
   | COND c t1 t2 => 
     match dev_cntr c e with
@@ -277,460 +81,24 @@ Fixpoint dev (f : Var -> Tree -> Cenv -> Tree)
     | CFALSE e      => dev f k t2 e
     | CBOTH c e1 e2 => COND c (dev f k t1 e1) (dev f k t2 e2)
     end
-  | CALL g args => f (maxn k (maxvar t)) t e
-    (*let: (t, xs) := get_func g p in
-      f (maxn k (maxvar t)) t (fmap_of xs (map e.1 args), e.2)*)
+  | CALL g args => f k t e
   end.
 
 Definition caller (f : Var -> Tree -> Cenv -> Tree) 
   (k : Var) (t : Tree) (e : Cenv) : Tree :=
   match t with
-  | CALL g args => let: (t, xs) := get_func g p in
-     f (maxn k (maxvar t)) t (fmap_of xs (map e.1 args), e.2)
-  | _ => '0
+  | CALL g args => 
+     let: (t, xs) := get_func g p in
+     f (maxn k (maxvar t)) t (mkEnv xs [seq x /s/ (e.1) | x <- args], e.2)
+  | _  => f k t e
   end.
 
-
-
-Lemma max_set0 : max_set fset0 = 0.
-Proof. by []. Qed.
-
-Lemma max_setin g x: 
-  x \in g -> x <= max_set g.
-Proof.
-elim: g=> //= a l IH; rewrite ?inE leq_max=> /orP[/eqP->|/IH->]; 
-by rewrite (leqnn, orbT).
-Qed.
-
-Lemma max_subset f g: {subset f <= g} -> max_set f <= max_set g.
-Proof.
-elim: f g=> //= a f IH g s; rewrite geq_max; apply/andP; split.
-- exact/max_setin/(s a)/mem_head.
-by apply/IH=> ? I; apply/s; rewrite inE I orbT.
-Qed.
-
-Lemma max_set_le {f h: {fset Var}} {k : Var}: 
-  max_set f <= k -> h `<=` f ->
-  max_set h <= k.
-Proof. move=> ? /fsubsetP /max_subset; slia.  Qed.
-
-Lemma max_add {f :{fset Var}} {k}: 
-  max_set f <= k -> max_set ([fset k.+1; k.+2] `|` f) <= k.+3.
-Proof.
-move=> ?. apply/(@leq_trans (max_set (k.+1 :: k.+2 :: f))).
-- apply/max_subset=> ?; by rewrite ?inE orbA.
-rewrite /= ?geq_max; apply/and3P; split; slia.
-Qed.
-
-Lemma foldr_monoid {T : Type} {f : T -> T -> T} {n s1 s2}: 
-  associative f ->
-  (forall x, f n x = x) ->
-  (forall x, f x n = x) ->
-  f (foldr f n s1) (foldr f n s2) =
-  foldr f n (s1 ++ s2).
-Proof. by move=> A L R; elim: s1=> //= ??; rewrite -A=>->. Qed.
-
-Lemma max_setU f g: 
-  max_set (f `|` g) = maxn (max_set f) (max_set g).
-Proof.
-have->: maxn (max_set f) (max_set g) = max_set (f ++ g).
-exact/(foldr_monoid maxnA max0n maxn0).
-have /andP/anti_leq //: ((max_set (f `|` g) <= max_set (f ++ g)) /\ 
-      (max_set (f ++ g) <= max_set (f `|` g)))%type.
-split; apply/max_subset=> ?; by rewrite ?inE mem_cat.
-Qed.
-
-
-Lemma max_set_le2 {f g h : {fset Var}} {k}: 
-  max_set f <= k -> max_set g <= k -> h `<=` f `|` g ->
-  max_set h <= k.
-Proof.
-move=> s1 s2 ?.
-by apply/(@max_set_le (f `|` g))=> //; rewrite max_setU geq_max s1 s2.
-Qed.
-
-Lemma mem_max_set f k:
-  max_set f <= k -> {in f, forall x, x <= k}.
-Proof. move=> ?? /max_setin; slia. Qed.
-
-Lemma mem_max_set' f k:
-  max_set f < k -> {in f, forall x, x < k}.
-Proof. move=> ?? /max_setin; slia. Qed.
-
-
-(*Definition dev_Prog (f : Prog) (e : seq Exp) := 
-  let: DEFINE n vs t := f in
-  let: s := size e in
-  DEFINE n (drop s vs) (dev (maxvar t) t (fmap_of vs e, [::])).*)
-
-Section SubstTh.
-
-Lemma substE (e1 e2 : Env) : 
-  (forall v : Var, v /s/ e1 = v /s/ e2) -> e1 = e2.
-Proof.
-by move=> E; apply/fsfunP=> [n]; move: (E n).
-Qed.
-
-Lemma substP (f : Exp -> Exp) (env : Env): 
-  (forall v : Var, env v = f v) ->
-  (forall a, f 'a = 'a) ->
-  (forall e1 e2, f (CONS e1 e2) = CONS (f e1) (f e2)) ->
-  (forall e, e /s/ env = f e).
-Proof.
-move=> ???; elim=> /= [[[]|?]|?->?->]//=.
-Qed.
-
-
-Lemma fsfunE {K : choiceType} {V : eqType} S f y dflt: 
-  ([fsfun x in S => f x] : {fsfun K -> V for dflt}) y = 
-  if y \in S then f y else dflt y.
-Proof. 
-rewrite /fsfun_of_fun /fsfun_of_ffun Fsfun.of_ffunE.
-by case: insubP=> [[/=??->->]|/negbTE->].
-Qed.
-
-Lemma emsubv (v : Var): 
-  emsub v = v.
-Proof. by rewrite fsfun_dflt /= ?finsupp0 ?inE. Qed.
-
-Lemma comp_env x e1 e2: 
-  x /s/ (comp e1 e2) = (x /s/ e1) /s/ e2.
-Proof.
-rewrite -[(x /s/ e1) /s/ e2]/((fun y => (y /s/ e1) /s/ e2) x).
-apply/substP=> // ?.
-rewrite /comp fsfunE; case: ifP=> //= /negbT.
-by rewrite inE negb_or => /andP[??]; rewrite fsfun_dflt //= fsfun_dflt.
-Qed.
-
-Lemma comp0e e1: comp emsub e1 = e1.
-Proof. by apply/substE=> v; rewrite comp_env /= emsubv. Qed.
-
-Lemma compe0 e1: comp e1 emsub = e1.
-Proof. 
-apply/substE=> v. rewrite comp_env /= -{2}[e1 v]/(id (e1 v)).
-apply/substP=> //; exact/emsubv.
-Qed.
-
-Lemma compA e1 e2 e3 : comp e1 (comp e2 e3) = comp (comp e1 e2) e3.
-Proof. by apply/substE=> ?; rewrite ?comp_env. Qed.
-
-Lemma subst_var (v u : Var) (e : Exp): 
-  v /s/ ([fsfun emsub with u |-> e]) = if v == u then e else v.
-Proof. by rewrite /= fsfun_withE emsubv. Qed.
-
-Lemma subst_fv e (e1 e2 : Env): 
-  (forall x, x \in FVExp e -> e1 x = e2 x) ->
-  e /s/ e1 = e /s/ e2.
-Proof.
-elim: e=> /= [[[]|?]|? IHe1 ? IHe2 H]//; first by (apply; rewrite ?inE).
-by apply/congr2; rewrite (IHe1, IHe2) // => ? I; rewrite H // ?inE I ?orbT.
-Qed.
-
-
-End SubstTh.
-
-Definition FVRestr (r : Restr) : {fset Var} := 
-  match r with
-  | NCONS v => FVArg v
-  | r1 ≠ r2 => FVArg r1 `|` FVArg r2
+Definition id_call (k : Var) (t : Tree) (c : Cenv):= 
+  let: (e, _) := c in
+  match t with
+  | CALL g args => CALL g [seq x /s/ e | x <- args]
+  | _ => t
   end.
-
-Section FreeValTh.
-
-Lemma finsupp_fsfun {s : {fset Var}} {f : Var -> Exp}: 
-  finsupp ([fsfun x in s => f x] : {fsfun Var -> Exp for id}) `<=` s.
-Proof.
-apply/fsubsetP=> ?; rewrite mem_finsupp fsfunE; case: ifP=> //.
-by rewrite eq_refl.
-Qed.
-
-Definition whole_env (e : Env)  := 
-  [fset x | a in finsupp e, x in FVExp (e a)].
-
-Lemma mem_whole_env x e: 
-  reflect (exists2 y, y \in finsupp e & (x \in FVExp (e y)))
-  (x \in whole_env e).
-Proof.
-apply/(iffP idP)=> [/imfset2P[y ? [? /[swap]<- ?]]|[y *]].
-- by exists y.
-apply/imfset2P; exists y=> //; by exists x.
-Qed.
-
-Definition whole_rs (rs : seq Restr) := 
-  [fset x | a in rs, x in FVRestr a].
-
-Lemma mem_whole_rs x rs: 
-  reflect (exists2 y, (y \in rs) & (x \in FVRestr y))
-  (x \in whole_rs rs).
-apply/(iffP idP)=> [/imfset2P[y ? [? /[swap]<- ?]]|[y *]].
-- by exists y.
-apply/imfset2P; exists y=> //; by exists x.
-Qed.
-
-Definition whole (e : Cenv) : {fset Var} :=
-  whole_env e.1 `|` whole_rs e.2.
-
-Lemma whole_env_substin (env : Env) v: 
-  v \in finsupp env ->
-  FVExp (env v) `<=` whole_env env.
-Proof. move=> ?; apply/fsubsetP=> ??; apply/mem_whole_env; by exists v. Qed.
-
-Lemma whole_env_subst (env : Env) (e : Exp): 
-  FVExp (e /s/ env) `<=` FVExp e `|` whole_env env.
-Proof.
-elim: e=> /= [[[]|v]|? IHe1 ? IHe2] //=.
-- case: (boolP (v \in finsupp env))=> [?|?].
-  apply/(fsubset_trans (whole_env_substin _ _ _))=> //.
-  by rewrite fsubsetUr.
-  by rewrite fsfun_dflt //= fsubsetUl.
-rewrite fsubUset; apply/andP; split.
-- apply/(fsubset_trans IHe1).
-  by rewrite [FVExp _ `|` FVExp _]fsetUC -fsetUA fsubsetUr.
-apply/(fsubset_trans IHe2); by rewrite -fsetUA fsubsetUr.
-Qed.
-
-
-Lemma whole_subst (env : Env) (rs : seq Restr) (e : Exp): 
-  FVExp (e /s/ env) `<=` FVExp e `|` whole (env, rs).
-Proof. by rewrite /whole fsetUA /= fsubsetU // whole_env_subst. Qed.
-
-Lemma whole_restr {e rs r}: 
-  whole (e, r :: rs) = FVRestr r `|` whole (e, rs).
-Proof.
-rewrite /whole /= fsetUC [whole_env _ `|` _]fsetUC fsetUA.
-apply/congr2=> //; apply/fsetP=> ?; rewrite inE.
-apply/(sameP idP)/(iffP idP)=> [/orP[]I|/mem_whole_rs[]].
-- apply/mem_whole_rs; exists r=> //=; by rewrite inE eq_refl.
-- case/mem_whole_rs: I=> y I *. apply/mem_whole_rs; exists y=> //.
-  by rewrite inE orbC I.
-move=> x; rewrite inE=> /orP[/eqP->-> //|??]; apply/orP; right.
-by apply/mem_whole_rs; exists x.
-Qed.
-
-Lemma whole_with {env : Env} {v : Var} {e : Exp} {rs}: 
-  whole ([fsfun env with v |-> e], rs) `<=` v |` (FVExp e) `|` whole (env, rs).
-Proof.
-rewrite -fsetUA fsubsetU //; apply/orP; right.
-rewrite /whole /= fsetUA fsetSU //.
-apply/fsubsetP=> ? /mem_whole_env[x].
-rewrite finsupp_with; case: ifP=> [/eqP->|].
-- rewrite fsfun_withE ?inE. case: ifP=> //= ???; apply/orP; right.
-  by apply/mem_whole_env; exists x.
-rewrite ?inE fsfun_withE; case: ifP=> //= [???->//|*]; apply/orP; right.
-by apply/mem_whole_env; exists x.
-Qed.
-
-Lemma comp_var (v : Var) env env': 
-  comp env env' v = (env v) /s/ env'.
-Proof. by rewrite -[comp env env' v]/(v /s/ (comp env env')) comp_env. Qed.
-
-
-Lemma whole_comp {env : Env} {v : Var} {e : Exp} {rs}: 
-  whole (comp env [fsfun emsub with v |-> e], rs) `<=` (FVExp e) `|` whole (env, rs).
-Proof.
-rewrite /whole /= fsetUA fsetSU //.
-apply/fsubsetP=> ? /mem_whole_env[x]; rewrite comp_var /comp.
-rewrite inE=> /(fsubsetP finsupp_fsfun); rewrite inE.
-case: (boolP (x \in finsupp env))=> /= [? _|?].
-- move/(fsubsetP (whole_env_subst _ _)); rewrite inE=> /orP[?|].
-  apply/orP; right; apply/mem_whole_env; by exists x.
-- case/mem_whole_env=> ?; rewrite finsupp_with; case: ifP=> [|?].
-  - by rewrite finsupp0 ?inE andbF.
-  by rewrite ?inE orbF=> /eqP->; rewrite fsfun_with=>->.
-rewrite finsupp_with; case: ifP; first by rewrite finsupp0 ?inE andbF.
-rewrite ?inE orbF fsfun_dflt // => ? /eqP-> /=.
-by rewrite fsfun_with=>->. 
-Qed.
-
-Lemma whole_cas {v a env rs}: 
-  whole (env, [seq cas v a i | i <- rs]) `<=`
-  FVArg a `|` whole (env, rs).
-Proof.
-rewrite /whole /= [FVArg _ `|` _]fsetUC -fsetUA fsetUS //.
-apply/fsubsetP=> x /mem_whole_rs[y /mapP[z]].
-rewrite /cas. case: z=> [r1 r2|].
-- case: ifP=> [/eqP->|].
-  - case: ifP=> [/eqP-> ? -> /=|]. 
-    - rewrite fsetUid inE=>->; by rewrite orbT.
-    move=> ?? -> /=; rewrite ?inE=> /orP[->|H]; first by rewrite orbT.
-    apply/orP; left; apply/mem_whole_rs; exists (v ≠ r2)=> //=.
-    by rewrite ?inE H orbT.
-  - case: ifP=> [/eqP-> ?? -> /=|].
-    - rewrite ?inE=> /orP[H|->]; last by rewrite orbT.
-    apply/orP; left; apply/mem_whole_rs; exists (r1 ≠ v)=> //=.
-    by rewrite ?inE H.
-  move=> ??? -> ?; rewrite ?inE.
-  apply/orP; left; apply/mem_whole_rs; by exists (r1 ≠ r2)=> //=.
-move=> u ? -> /= ?; rewrite ?inE.
-apply/orP; left; apply/mem_whole_rs; by exists (NCONS u)=> //=.
-Qed.
-
-Definition aux (e : Env) (f : {fset Var}): {fset Var} :=
-  [fset x | a in f, x in FVExp (e a)].
-
-Lemma mem_aux (e : Env) (f : {fset Var}) x: 
-  reflect (exists2 y, y \in f & x \in FVExp (e y))
-  (x \in aux e f).
-Proof.
-apply/(iffP idP)=> [/imfset2P[y ? [? /[swap]-> ?]]|[y ??]].
-- by exists y.
-apply/imfset2P; exists y=> //; by exists x.
-Qed.
-
-Lemma auxU f g e: aux e (f `|` g) = aux e f `|` aux e g.
-Proof.
-apply/fsetP=> ?; apply/(sameP idP)/(iffP idP); rewrite ?inE.
-- by case/orP=> /mem_aux[x I ?]; apply/mem_aux; exists x=> //; rewrite ?inE I ?orbT.
-case/mem_aux=> x.
-by rewrite ?inE=> /orP[] I ?; apply/orP; [left | right]; apply/mem_aux; exists x.
-Qed.
-
-Lemma aux_FVExp e a : aux e (FVExp a) = FVExp a /s/ e.
-Proof.
-elim: a=> [|? IH1 ? IH2] /=; last by rewrite auxU IH1 IH2.
-- case=> [[]?|v] //=; apply/fsetP=> ?; apply/(sameP idP)/(iffP idP).
-  - by rewrite inE.
-  - case/mem_aux=> ?; by rewrite inE.
-  - move=> ?; apply/mem_aux; exists v=> //; by rewrite ?inE.
-  by case/mem_aux=> ?; rewrite ?inE=> /eqP->.
-Qed.
-
-
-Lemma aux_CONS e a: 
-  aux e (FVCntr (CONS? a)) = FVExp (a /s/ e).
-Proof.
-move=> /=; have->: FVArg a = FVExp a by case: a=> [[]|].
-exact/aux_FVExp.
-Qed.
-
-Lemma aux_EQA e a1 a2: 
-  aux e (FVCntr (EQA? a1 a2)) = FVExp (a1 /s/ e) `|` FVExp (a2 /s/ e).
-Proof. by move=> /=; rewrite auxU ?aux_FVExp. Qed.
-
-Lemma auxE e c rs: 
-  aux e (FVCntr c) `<=` FVCntr c `|` whole (e, rs).
-Proof.
-apply/fsubsetP=> y /mem_aux[x I]. 
-rewrite -[e x]/((Exp_Arg (Arg_Var x)) /s/ e)=> /(fsubsetP (whole_subst _ rs _)).
-move=> /=; rewrite 2?inE => /orP[/eqP->|H]; first by rewrite inE I.
-by rewrite inE H orbT.
-Qed.
-
-Lemma memNwhole k rs v env env'  e1 l: 
-  max_set (whole (env, rs)) <= k ->
-  v < l -> k < l ->
-  (env v) /s/ [fsfun env' with l |-> e1] = 
-  (env v) /s/ env'.
-Proof.
-move/mem_max_set=> m ??.
-case: (boolP (v \in finsupp env))=> [/whole_env_substin H|?].
-- have: forall x, x \in FVExp (env v) -> x <= k.
-  move=> ? /(fsubsetP H) I; apply/m; by rewrite inE /= I.
-  elim: (env v)=> [[[]|u /(_ _ (fset11 _))]|] //=.
-  - rewrite fsfun_withE; case: ifP; slia.
-  move=> ? IHe1 ? IHe2 I; rewrite IHe1 ?IHe2 //; 
-  by move=> ? I'; apply/I; rewrite ?inE I' ?orbT.
-rewrite fsfun_dflt //= fsfun_withE; case: ifP; slia.
-Qed.
-
-Lemma whole_cons rs (env : Env) (v : Var) e1 e2: 
-  env v = CONS e1 e2 -> 
-  ((FVExp e1 `<=` whole (env, rs)) * (FVExp e2 `<=` whole (env, rs)))%type.
-Proof.
-case: (boolP (v \in finsupp env))=> [/whole_env_substin|?].
-- move=> /[swap]-> /=; rewrite fsubUset /whole /= => /andP[H1 H2].
-  by rewrite ?fsubsetU // (H1, H2).
-by rewrite fsfun_dflt.
-Qed.
-
-End FreeValTh.
-
-Section ContradictTh.
-
-Lemma cont_isCONS rs v: contradict rs (isCONS v) = (NCONS v \in rs).
-Proof.
-elim: rs=> //= a ?; rewrite inE /contr; case: a=> // a ->; apply/orb_id2r=> ?.
-by apply/(sameP _ eqP)/(iffP eqP)=> [|[]]->.
-Qed.
-
-Lemma cont_isEQ rs v u: 
-  reflect (exists r1 r2, r1 ≠ r2 \in rs /\
-  ((r1, r2) = (v, u) \/ (r2, r1) = (v, u)))
-  (contradict rs (isEQ v u)).
-Proof. 
-apply/(iffP hasP)=> [[[]//= r1 r2 ?]|[r1 [r2 [?]]]] /pred2P ?.
-- by exists r1, r2.
-by exists (r1 ≠ r2).
-Qed.
-
-Lemma Ncont_isEQ rs v u: 
-  reflect (forall r1 r2, r1 ≠ r2 \in rs ->
-  ((r1, r2) <> (v, u) /\ (r2, r1) <> (v, u)))
-  (~~ (contradict rs (isEQ v u))).
-Proof.
-apply/(iffP hasPn)=> [H ?? /H|H []// ?? /H[/eqP/[swap]/eqP]]; rewrite negb_or.
-- by case/andP=>/eqP?/eqP.
-by move->=>->.
-Qed. 
-
-Lemma ncontr_cons e rs v: 
-  ncontr_env e (NCONS v :: rs) <->
-  (ncontr_env e rs /\ ncontr_ncons e v).
-Proof.
-split=> [][] H1 H2; do ?split.
-- by move=> ?? I; apply/H1; rewrite ?inE I orbT.
-- by move=> ? I; apply/H2; rewrite ?inE I orbT.
-- by apply/H2; rewrite ?inE eq_refl.
-- by move=> ??; rewrite inE=> /orP[]//; case: H1=> H ? /H.
-by move=> ?; rewrite inE=> /orP[/eqP[->]|]//; case: H1=> ? H /H.
-Qed.
-
-Lemma ncontr_eq e rs v u: 
-  ncontr_env e (v ≠ u :: rs) <->
-  (ncontr_env e rs /\ ncontr_neq e v u).
-Proof.
-split=> [][] H1 H2; do ?split.
-- by move=> ?? I; apply/H1; rewrite ?inE I orbT.
-- by move=> ? I; apply/H2; rewrite ?inE I orbT.
-- by apply/H1; rewrite ?inE eq_refl.
-- by move=> ??; rewrite inE=> /orP[/eqP[->->]|]//; case: H1=> H ? /H.
-by move=> ?; rewrite inE=> /orP[]//; case: H1=> ? H /H.
-Qed.
-
-Lemma ncontr_whole env' env v rs e: 
-  max_set (whole (env', rs)) < v ->
-  ncontr_env env rs ->
-  ncontr_env [fsfun env with v |-> e] rs.
-Proof.
-move/mem_max_set'=> H.
-have: {in whole_rs rs, forall x : nat, x < v}=> [? I|{H}H].
-- by apply/H; rewrite /whole /= ?inE I orbT.
-case=> H1 H2; split=> [r1 r2 I|].
-  - have: {subset FVRestr (r1 ≠ r2) <= whole_rs rs}.
-    move=> ??; apply/mem_whole_rs; by exists (r1 ≠ r2).
-  case: r1 r2 I=> [[? [[? /H1 //]|u /H1 N I]]|] /=.
-  - have ?: u < v.
-    - by apply/H/I=> /=; rewrite ?inE eq_refl.
-    move=> ? /= /[dup] ?; rewrite fsfun_withE; case: ifP; try slia.
-    move=> *; exact/N.
-  move=> u [[? /H1 N I]|] /=.
-    - have ?: u < v by apply/H/I=> /=; rewrite ?inE eq_refl.
-      move=> /[swap] ? /= /[dup] ?; rewrite fsfun_withE; case: ifP; try slia.
-    move=> *; exact/N.
-  move=> u' /H1 N I .
-  - have ?: u < v by apply/H/I=> /=; rewrite ?inE eq_refl.
-  - have ?: u' < v by apply/H/I=> /=; rewrite ?inE eq_refl orbT.
-  move=> /[dup] ? /[dup] ? /=; rewrite ?fsfun_withE; do ?case: ifP; try slia.
-  move=> *; exact/N.
-move=> [[]|] // u I.
-have: {subset FVRestr (NCONS u) <= whole_rs rs}.
-move=> ??; apply/mem_whole_rs; by exists (NCONS u).
-move: I=> /[swap] /= I /H2 N.
-- have ? : u < v by apply/H/I; rewrite ?inE eq_refl.
-rewrite /ncontr_ncons /= fsfun_withE; case: ifP; slia.
-Qed.
-
-End ContradictTh.
 
 Arguments FVCntr : simpl never.
 
@@ -961,107 +329,20 @@ case: (_ /s/ e1)=> [[[]|]|???+[<-]] /=.
 by case: (e2 _).
 Qed.
 
-Fixpoint well_typed (t : Tree) : bool := 
-  match t with 
-  | RET _ => true
-  | LET v x t => well_typed t && (v \notin FVExp x)
-  | COND c t1 t2 =>  well_typed t1 && well_typed t2 
-  | HT v u x t => [&& x != v, x != u, v != u & well_typed t]
-  | CALL f xs => size xs == size (get_func f p).2
-  end.
-
 Arguments whole : simpl never.
 
-Lemma subst_max (e1 e2 : Env) (e : Exp) : 
-  (forall x, x <= maxvar e -> e1 x = e2 x) ->
-  e /s/ e1 = e /s/ e2.
-Proof.
-elim: e=> [[[]|?]|? IHe1 ? IHe2 I] //=; first apply.
-- rewrite /maxvar /=; apply/max_setin; by rewrite ?inE.
-  by rewrite IHe1 ?IHe2 //; move=> ? I'; apply/I; rewrite /maxvar /=;
-rewrite max_setU leq_max I' ?orbT.
-Qed.
+Notation well_typed := (@well_typed p).
+
 
 Definition correct (f : Var -> Tree -> Cenv -> Tree) := 
-  forall e1 e2 rs k n g args,
+  forall e1 e2 rs k g args n ,
   let: t := CALL g args in 
-  int n t (comp e1 e2) p <> '0 ->
+  int n t (comp e1 e2) p <> ERROR ->
   well_typed t -> 
   max_set (whole (e1, rs)) <= k ->
   maxvar t <= k ->
   ncontr_env e2 rs ->
   int n t (comp e1 e2) p = int n (f k t (e1, rs)) e2 p.
-
-Lemma int_freevar (e1 e2 : Env) t n: 
-  well_typed t ->
-  (forall x, x \in FVTree t -> e1 x = e2 x) ->
-  int n t e1 p = int n t e2 p.
-Proof.
-elim: t e1 e2 n=> [??? n ? H *|??? IHt ?? n|c ? IHt1 ? IHt2 ++ n|?? v ? IHt e1 e2 n|++++ n].
-all: case: n=> // n.
-- apply/subst_fv=> *; exact/H.
-- move=> /andP[? /negbTE NI I]; apply/IHt=> // ? F; rewrite ?fsfun_withE.
-  case: ifP=> [/eqP E|N].
-  - apply/subst_fv=> ? I'; apply/I; rewrite /= ?inE I' /= andbT.
-    apply/negP=> /eqP E'; by rewrite E' NI in I'.
-  by apply/I; rewrite ?inE F N orbT.
-- case: c=> [[[a ?? /andP[??] I]|v e1 e2 /andP[??] I]|] /=.
-  - apply/IHt2=> // ? I'; apply/I; by rewrite ?inE I' orbT.
-  - have->: e1 v = e2 v by apply/I; rewrite ?inE eq_refl.
-    case E: (e2 v); [apply/IHt2 | apply/IHt1] => // ? I'; apply/I;
-    by rewrite ?inE I' orbT.
-  - move=> e e' e1 e2 /andP[??] I.
-    have->: (e /s/ e1 = e /s/ e2). 
-    - by apply/subst_fv=> ? I'; apply/I; rewrite ?inE I'.
-    case: (e /s/ e2)=> // [[[]|]] //= ?.
-    have->: (e' /s/ e1 = e' /s/ e2).
-    - by apply/subst_fv=> ? I'; apply/I; rewrite ?inE I' orbT.
-    case: (e' /s/ e2)=> // [[]] // [?]; case: ifP=> ?;
-    [apply/IHt1 | apply/IHt2] => // ? I'; apply/I; by rewrite ?inE I' ?orbT.
-- case/and4P=> N1 N2 ?? I /=.
-  have->: e1 v = e2 v.
-  - by apply/I=> /=; rewrite ?inE N1 N2 eq_refl /=.
-  case: (e2 v)=> // ??; apply/IHt=> // ? I'; rewrite ?fsfun_withE.
-  (do? case: ifP=> //)=> N1' N2'; apply/I; by rewrite ?inE N1' N2' I' orbT.
-move=> f l e1 e2 ? IH /=.
-case: (get_func f p)=> ? xs.
-have-> //: (fmap_of xs [seq e1 i | i <- l]) =  (fmap_of xs [seq e2 i | i <- l]).
-apply/congr1/eq_in_map=> ? H. apply/IH; by rewrite seq_fsetE.
-Qed.
-
-Lemma int_maxvar (e1 e2 : Env) t n: 
-  well_typed t ->
-  (forall x, x <= maxvar t -> e1 x = e2 x) ->
-  int n t e1 p = int n t e2 p.
-Proof.
-move=> wf H; apply/int_freevar=> // ? I; rewrite H // /maxvar max_setin //.
-elim: t I {wf H}=> //= [??? IH|?? IH1 ? IH2|???? IH]; rewrite ?inE.
-- case/andP=> ? /orP[|/IH]->; by rewrite ?orbT.
-- case/orP=> [/orP[|/IH1]|/IH2]->; by rewrite ?orbT.
-case/and3P=> ?? /orP[|/IH]->; by rewrite ?orbT.
-Qed.
-
-Arguments int: simpl nomatch.
-
-Lemma int_not0 n t e: 
-  int n t e p <> '0 ->
-  int n t e p = int n.+1 t e p.
-Proof.
-elim: n t e p=> [[]|] // n IH [] //=.
-- move=> *; by rewrite IH.
-- move=> c ?? e ?; case: c=> //= [[[]??|v]|] //=; rewrite 1?IH //;
-  rewrite /int /= -/int.
-  - case E: (e v)=> ?; by rewrite IH.
-  move=> e1 e2 /=. case: (e1 /s/ e)=> //= [[]] // [] //.
-  case (e2 /s/ e)=> [] // [] // [] ??; case: ifP=> ??; by rewrite IH.
-- move=> ?? v ?; rewrite /int/= -/int=> e; case: (e v)=> // *.
-  by rewrite IH.
-move=> ????. rewrite {1 2 3}/int/=-/int. case: (get_func _ _)=> // ???.
-by rewrite IH.
-Qed.
-
-Lemma l k: (k.+2 == k.+1) = false.
-Proof. by apply/eqP=> /esym /n_Sn. Qed.
 
 Arguments int : simpl never.
 
@@ -1069,23 +350,17 @@ Hypothesis well_typed_prog : forall f,
   ((well_typed (get_func f p).1) *
   ({subset FVTree (get_func f p).1 <= (get_func f p).2}))%type.
 
-Lemma whole_fmap {xs} {e : Env} {l rs}: 
-  whole (fmap_of xs (map e l), rs) `<=` 
-  whole (e, rs) `|` (seq_fset tt l).
-Proof. Admitted.
-
-Lemma fmap_of0 xs: fmap_of xs [::] = emsub.
-Proof. by case: xs. Qed.
-
-Lemma fmap_ofcons v vs x xs: fmap_of (x :: xs) (v :: vs) = 
-  [fsfun fmap_of xs vs with x |-> v].
-Proof. by []. Qed.
-
-
-Lemma correct_dev f : 
-  correct f -> correct (dev f).
+Lemma int_dev f e1 e2 rs k t n: 
+  correct f ->
+  int n t (comp e1 e2) p <> ERROR ->
+  well_typed t -> 
+  max_set (whole (e1, rs)) <= k ->
+  maxvar t <= k ->
+  ncontr_env e2 rs ->
+  int n t (comp e1 e2) p = int n (dev f k t (e1, rs)) e2 p.
 Proof.
-move=> corr * e1 e2 rs k t.
+have l: forall k, (k.+2 == k.+1) = false by slia.
+move=> corr; move: n. 
 elim: t e1 e2 rs k => // [/= +++++ n|/= v e t IHt e1 e2 rs k n|||].
 1,2: case: n=> //.
 - move=> *. by rewrite /int /= comp_env.
@@ -1187,129 +462,152 @@ rewrite -?fsetUA fsetUS // fsubUset; apply/andP; split.
 - apply/(fsubset_trans H2); by rewrite fsetUA fsubsetUr.
 by rewrite fsetUA fsubsetUr.
 apply/(max_set_le m)=> /=; by rewrite fsubsetUr.
+move=> g ? e1 e2 ?? [] //= n *.
+by rewrite -corr.
+Qed.
 
-move=> g l e1 e2 ?? [] // n. rewrite {1 2}/int -/int /=.
-case E: (get_func g)=> [vs xs]; rewrite /maxvar => N /eqP ++ m2.
-move=> /= S  m1 ?.
+Lemma correct_dev f : 
+  correct f -> correct (caller (dev f)).
+Proof.
+move=> corr e1 e2 rs k g l /= [] //=.
+rewrite {1 2}/int /= -/int; case E: (get_func g p)=> [vs xs] //=.
+rewrite /maxvar => n N /eqP ++ m2; move=> /= S  m1 ?.
 have ?: well_typed vs by rewrite -[vs]/((vs, xs).1) -E well_typed_prog.
 have H: 
-  int n vs (fmap_of xs [seq comp e1 e2 i | i <- l]) p =
-  int n.+1 vs (comp (fmap_of xs [seq e1 i | i <- l]) e2) p.
-- rewrite int_not0 //; apply/int_freevar=> // x.
+  int n vs (mkEnv xs [seq x /s/ (comp e1 e2) | x <- l]) p =
+  int n.+1 vs (comp (mkEnv xs [seq x /s/ e1 | x <- l]) e2) p.
+- rewrite int_not0 //; apply/int_freevar => // x.
   case: (well_typed_prog g)=> ?; rewrite E /==> /[apply].
   elim: xs l {E N m2} S=> //= ?? IHxs [] //= ?? [/IHxs IH].
   rewrite ?fmap_ofcons ?inE ?comp_var ?fsfun_withE.
-  case: ifP=> //= ? /IH->; by rewrite comp_var.
-rewrite -corr -?H ?leq_max /maxvar ?leqnn ?orbT // => //=.
+  case: ifP=> //=; first by rewrite comp_env.
+  move=> ? /IH->; by rewrite comp_var.
+rewrite -int_dev ?leq_max ?leqnn ?orbT // -?H //.
 by apply/orP; left; apply/(max_set_le2 m1 m2)/(fsubset_trans whole_fmap).
 Qed.
 
-Lemma correct_devn f n: correct f ->
-  correct (iter n dev f).
-Proof. by elim: n=> // ? /[apply] /correct_dev. Qed.
+
+
+Lemma correct_id: correct id_call.
+Proof.
+move=> ???? g l [] //= ? N /eqP S ? m *; rewrite /int/=-/int.
+case E: (get_func g p)=> [t xs]. 
+have ?: well_typed t by rewrite -[t]/((t, xs).1) -E well_typed_prog.
+apply/int_freevar=> //; rewrite -[t]/((t, xs).1) -?E=> ? /=.
+case: (well_typed_prog g)=> ? /[apply]; rewrite E /=.
+rewrite E /= in S.
+elim: xs l {E N m} S=> //= ?? IHxs [] //= ?? [/IHxs IH].
+rewrite ?fmap_ofcons ?inE ?comp_var ?fsfun_withE.
+case: ifP=> //; by rewrite comp_env.
+Qed.
+
+Definition devn n := iter n (caller \o dev) id_call.
+
+Lemma correct_devn n:
+  correct (devn n).
+Proof. elim: n=> [|?]; [exact/correct_id | exact/correct_dev]. Qed.
 
 End Spec.
 
-Definition int_Prog n (main : Prog) (p : Programm) (xs : seq Exp) : Exp := 
+Definition int_Prog n (main : Def) (p : Prog) (xs : seq Exp) : Exp := 
   let: DEFINE f vs t := main in 
-    int n t (fmap_of vs xs) p.
+    int n t (mkEnv vs xs) p.
 
-Definition dev_Prog f (p : Programm) (xs : seq Exp) : Prog := 
-  match p with
-  | [::]   => DEFINE 0 [::] (RET '0)
-  | (DEFINE g vs t) :: _ => 
-    let: cenv := (fmap_of vs xs, [::]) in 
-    DEFINE g (drop (size xs) vs)
-        (dev p f (maxn (maxvar t) (max_set (whole cenv))) t cenv)
-  end.
+Definition spec f (main : Def) (xs : seq Exp) : Def := 
+  let: DEFINE g vs t := main in 
+  let: cenv := (mkEnv vs xs, [::]) in 
+  let t' := (CALL g (map (Exp_Arg \o Arg_Var) vs)) in
+  DEFINE g (drop (size xs) vs) (f 
+    (maxn (maxvar t') (max_set (whole cenv)))
+   t'
+    cenv
+  ).
 
 Definition well_typed_prog p := 
   forall f,
-  ((well_typed p (get_func f p).1) *
+  ((@well_typed p (get_func f p).1) *
   ({subset FVTree (get_func f p).1 <= (get_func f p).2}))%type.
 
 
-Lemma fmap_cat e1 e2 t:
-  (forall x, x \in e1 -> closed x) ->
-  (forall x, x \in e2 -> closed x) ->
-  size t = (size e1 + size e2)%N  ->
-  fmap_of t (e1 ++ e2) =
-  comp (fmap_of t e1) (fmap_of (drop (size e1) t) e2).
+Lemma int_call n t f vs e p: 
+  well_typed_prog (DEFINE f vs t :: p) ->
+  int n t e (DEFINE f vs t :: p) = 
+  int n.+1 (CALL f [seq (Exp_Arg \o Arg_Var) i | i <- vs]) e (DEFINE f vs t :: p).
 Proof.
-Admitted.
-(*  move=> E.
-  rewrite /fmap_of (foldr_monoid compA comp0e compe0); apply/congr1.
-  rewrite -map_cat -{1}(cat_take_drop (size e1) t) zip_cat.
-  apply/congr1/congr2=> //.
-  - rewrite -{3}(cats0 e1) -{2}(cat_take_drop (size e1) t) zip_cat.
-    by case: (drop _)=> /=; rewrite cats0.
-all: by rewrite size_takel // E -{1}(addn0 (size e1)) leq_add2l leq0n. 
-Qed.*)
+move=> wf.
+case: n=> [/=|/=n]; rewrite ?eq_refl; first by case: t wf.
+apply: (int_freevar _ _ _ n.+1); move: (wf f); rewrite /=eq_refl/==> [[]] //.
+move=> _ /[swap] ? /[apply].
+elim: vs  {wf}=> //= ??.
+by rewrite fmap_ofcons ?inE fsfun_withE; case: ifP=> // /eqP->.
+Qed.
 
-Theorem int_dev_Prog (p : Programm) (main : Prog) (e1 e2 : seq Exp) f:
+Arguments int : simpl nomatch.
+
+
+Lemma int_spec (p : Prog) (main : Def) (e1 e2 : seq Exp) f:
   let: (DEFINE _ vs main_t) := main in
   (size e1 + size e2)%N = size vs ->
   (forall x, x \in e1 -> closed x) ->
-  (forall x, x \in e2 -> closed x) ->
   well_typed_prog (main :: p) ->
-  well_typed (main :: p) main_t ->
   correct (main :: p) f ->
   forall n,
-  int_Prog n main (main :: p) (e1 ++ e2) <> '0 ->
+  int_Prog n main (main :: p) (e1 ++ e2) <> ERROR ->
   int_Prog n main (main :: p) (e1 ++ e2) = 
-  int_Prog n (dev_Prog f (main :: p) e1) (main :: p) e2.
+  int_Prog n.+1 (spec f main e1) (main :: p) e2.
 Proof. 
-case: main => /= ? l ? H ???? n ?.
-by rewrite fmap_cat //= => ?; rewrite -correct_dev // leq_max leqnn ?orbT.
+case: main => /= ? l ? H ?? corr n.
+rewrite fmap_cat //= => ?. 
+by rewrite -corr -?int_call //= ?eq_refl /= ?size_map // leq_max ?leqnn ?orbT.
+Qed.
+
+Definition specn m f e p := 
+     spec (devn (f :: p) m) f e.
+
+Arguments specn /.
+
+Theorem int_devn_Prog (p : Prog) (main : Def) (e1 e2 : seq Exp) m:
+  let: (DEFINE _ vs main_t) := main in
+  (size e1 + size e2)%N = size vs ->
+  (forall x, x \in e1 -> closed x) ->
+  well_typed_prog (main :: p) ->
+  forall n,
+  int_Prog n main (main :: p) (e1 ++ e2) <> ERROR ->
+  int_Prog n main (main :: p) (e1 ++ e2) = 
+  int_Prog n.+1 (specn m main e1 p) (main :: p) e2.
+Proof.
+case: main=> *. 
+apply/(int_spec p (DEFINE _ _ _))=> //.
+exact/correct_devn.
 Qed.
 
 Definition x1  : Var := 1.
 Definition x2  : Var := 2.
 Definition yes : Val := '3.
 Definition no  : Val := '4.
-
-Notation "'If' c 'Then' t1 'Else' t2" := (COND c t1 t2) (at level 30).
-
-Definition cons_cons : Programm := 
-  [::
-    DEFINE 1 [:: x1; x2] 
-      (If (CONS? x1) Then
-        If (CONS? x2) Then
-          yes
-        Else no
-      Else
-        If (CONS? x2) Then
-          no
-        Else yes)
-  ].
-
-Lemma dev_cons_cons f: 
-  dev_Prog f cons_cons [:: CONS '3 '4] = 
-  DEFINE 1 [:: x2] (If (CONS? x2) Then yes Else no).
-rewrite /cons_cons /= /fmap_of /= ?comp_var ?fsfun_with /= ?comp_var fsfun_withE.
-have->: x2 == x1 = false by slia.
-by rewrite ?emsubv /= ?emsubv.
-Qed.
-
 Definition h1 : Var := 3.
 Definition h2 : Var := 4.
 Definition t1 : Var := 5.
 Definition t2 : Var := 6.
 
+Notation "'If' c 'Then' t1 'Else' t2" := (COND c t1 t2) (at level 100).
+Notation "h : t <- x" := (HT h t x) (at level 10).
 
-Definition eq_tree : Programm := 
-  [::
+
+(*Arguments calling : simpl never.*)
+
+Definition eq_tree : Def := 
     DEFINE 1 [:: x1; x2] (
         If (CONS? x1) Then
-          (HT h1 t1 x1 (
+          h1 : t1 <- x1 (
             If (CONS? x2) Then
-              (HT h2 t2 x2 (
+              h2 : t2 <- x2 (
                 If (EQA? h1 h2) Then
-                  CALL 1 [:: t1; t2]
+                  CALL 1 [:: Exp_Arg (Arg_Var t1); Exp_Arg (Arg_Var t2)]
                 Else no
-              ))
+              )
             Else no
-          ))
+          )
         Else 
           If (CONS? x2) Then
             no
@@ -1317,15 +615,4 @@ Definition eq_tree : Programm :=
             If (EQA? x1 x2) Then 
               yes
             Else no
-      )
-  ].
-
-Definition deveq_tree f := iter 10 (dev eq_tree) f.
-Arguments deveq_tree : simpl never.
-
-Lemma dev_eq_tree f: 
-  dev_Prog (deveq_tree f) eq_tree [:: CONS '3 '4] = 
-  DEFINE 0 [::] (RET '0).
-Proof.
-rewrite /eq_tree /=.
-
+      ).
