substitution.v
@@ -1,0 +1,592 @@
+From mathcomp Require Import ssreflect ssrnat eqtype ssrbool ssrfun seq.
+From mathcomp Require Import finmap choice finfun fintype.
+From deriving Require Import deriving.
+From coqspec Require Import utilities.
+
+Set Implicit Arguments.
+Unset Printing Implicit Defensive.
+
+Open Scope fmap_scope.
+Open Scope fset_scope.
+Definition Atom  := nat.
+Definition Var  := nat.
+Definition FName := nat.
+
+Inductive Val := ATOM of Atom.
+Notation "''' e" := (ATOM e) (at level 0).
+
+Notation "'ERROR'" := ('0) (only parsing).
+
+Definition val_indDef := [indDef for Val_rect].
+Canonical val_indType := IndType Val val_indDef.
+
+Definition val_eqMixin := [derive eqMixin for Val].
+Canonical val_eqType := EqType Val val_eqMixin.
+Definition val_choiceMixin := [derive choiceMixin for Val].
+Canonical val_choiceType := Eval hnf in ChoiceType Val val_choiceMixin.
+
+Inductive Arg := 
+  | Arg_Val of Val
+  | Arg_Var of Var.
+Coercion Arg_Val : Val >-> Arg.
+Coercion Arg_Var : Var >-> Arg.
+
+Definition arg_indDef := [indDef for Arg_rect].
+Canonical arg_indType := IndType Arg arg_indDef.
+
+Definition eq_arg a b := 
+  match a, b with
+  | Arg_Val 'a, Arg_Val 'b => a == b
+  | Arg_Var x, Arg_Var y => x == y
+  | _, _ => false
+  end.
+
+Lemma eqargP : Equality.axiom eq_arg.
+Proof. 
+by case=> [[]?[[]|]|?[]]?/=; try (by constructor); apply/(iffP eqP)=> [|[]]->. 
+Qed.
+
+Canonical arg_eqMixin := EqMixin eqargP.
+Canonical arg_eqType := Eval hnf in EqType Arg arg_eqMixin.
+
+Definition arg_choiceMixin := [derive choiceMixin for Arg].
+Canonical arg_choiceType := Eval hnf in ChoiceType Arg arg_choiceMixin.
+
+Inductive Exp :=
+  | Exp_Arg of Arg
+  | CONS of Exp & Exp.
+Coercion Exp_Arg : Arg >-> Exp.
+
+Fixpoint eq_exp a b := 
+  match a, b with
+  | Exp_Arg a,  Exp_Arg b  => a == b
+  | CONS e1 e2, CONS e3 e4 => eq_exp e1 e3 && eq_exp e2 e4
+  | _,          _          => false
+  end.
+
+Lemma eqexpP : Equality.axiom eq_exp.
+Proof.
+elim=> [?[]*|? IHe1 ? IHe2[]]/= *; first by apply/(iffP eqP)=> [|[]]//->.
+1,2: by constructor.
+by apply/(iffP andP)=> [][]/IHe1->/IHe2->.
+Qed.
+
+Canonical exp_eqMixin := EqMixin eqexpP.
+Canonical exp_eqType := Eval hnf in EqType Exp exp_eqMixin.
+
+Definition exp_indDef := [indDef for Exp_rect].
+Canonical exp_indType := IndType Exp exp_indDef.
+
+Definition exp_choiceMixin := [derive choiceMixin for Exp].
+Canonical exp_choiceType := Eval hnf in ChoiceType Exp exp_choiceMixin.
+
+Definition Env := {fsfun Var -> Exp for id}.
+
+Fixpoint subst (e : Exp) (env : Env) : Exp := 
+  match e with 
+  | CONS e1 e2 => CONS (subst e1 env) (subst e2 env)
+  | 'a         => 'a
+  | (Exp_Arg (Arg_Var v))      =>  env v 
+  end.
+
+Notation "e '/s/' env" := (subst e env) (at level 1, left associativity).
+
+Arguments subst : simpl nomatch.
+
+Definition comp (e1 e2 : Env) : Env := 
+  [fsfun x in (finsupp e1 `|` finsupp e2) => (e1 x) /s/ e2].
+
+Definition emsub : Env := [fsfun for (id : Var -> Exp)].
+
+Definition mkEnv (ks : seq Var) (vs : seq Exp) : Env :=
+  foldr (fun '(v, x) a => [fsfun a with v |-> x]) emsub (zip ks vs).
+
+Fixpoint FVExp (e : Exp) : {fset Var} := 
+  match e with
+  | CONS e1 e2 => FVExp e1 `|` FVExp e2
+  | (Exp_Arg (Arg_Var v))      => [fset v]
+  | _          => fset0
+  end.
+
+Definition closed e := FVExp e == fset0.
+
+Definition FVArg (a : Arg) := 
+  if a is (Arg_Var x) then [fset x] else fset0.
+
+Definition closed_sub (e : Env) := 
+  forall x, x \in finsupp e -> closed (e x).
+
+Inductive Restr := 
+  | Neq of Arg & Arg
+  | NCONS of Arg.
+
+Definition restr_indDef := [indDef for Restr_rect].
+Canonical restr_indType := IndType Restr restr_indDef.
+
+Definition restr_eqMixin := [derive eqMixin for Restr].
+Canonical restr_eqType := Eval hnf in EqType Restr restr_eqMixin.
+
+Definition restr_choiceMixin := [derive choiceMixin for Restr].
+Canonical restr_choiceType := Eval hnf in ChoiceType Restr restr_choiceMixin.
+
+Notation "e1 '≠' e2" := (Neq e1 e2) (at level 10).
+
+Definition Cenv := (Env * seq Restr)%type.
+
+Definition FVRestr (r : Restr) : {fset Var} := 
+  match r with
+  | NCONS v => FVArg v
+  | r1 ≠ r2 => FVArg r1 `|` FVArg r2
+  end.
+
+
+Inductive Bind :=
+  | isEQ of Arg & Arg
+  | isCONS of Arg.
+
+Definition contr  (b : Bind) (r : Restr) := 
+  match r, b with
+  | v ≠ u, isEQ v' u' => ((v, u) == (v', u')) || ((u, v) == (v', u'))
+  | NCONS v, isCONS u => v == u
+  | _, _              => false
+  end.
+
+Definition is_arg (e : Exp) := 
+  if e is Exp_Arg _ then true else false.
+
+Definition is_cons (e : Exp) := 
+  if e is CONS _ _ then true else false.
+
+
+Definition ncontr_neq env r1 r2 := 
+    is_arg (r1 /s/ env) ->
+    is_arg (r2 /s/ env) ->
+    r1 /s/ env <> r2 /s/ env.
+
+Definition ncontr_ncons env r := 
+  ~~ is_cons (r /s/ env).
+
+
+Definition ncontr_env (env : Env) (rs : seq Restr) := 
+  (forall r1 r2, r1 ≠ r2 \in rs -> ncontr_neq env r1 r2) /\
+  (forall r, NCONS r \in rs -> ncontr_ncons env r).
+
+
+Definition contradict r b : bool :=
+  has (contr b) r .
+
+Definition delete_restr (v : Var) := 
+  filter (fun r => match r with 
+                   | (r1 ≠ r2) => (r1 != v) && (r2 != v)
+                   | NCONS r => r != v
+                  end).
+
+Definition cas  (v u : Arg) (r : Restr) := 
+  if r is x ≠ y then 
+    (if x == v then u else x) ≠ (if y == v then u else y)
+  else r.
+
+
+Definition rsubst (r : seq Restr) (b : Bind) : seq Restr := 
+  match b with 
+  | isEQ u v => map (cas u v) r
+  | isCONS _ => r
+  end.
+
+Definition of_Bind b : Env := 
+  match b with 
+  | isEQ (Arg_Var u) v => [fsfun emsub with u |-> Exp_Arg v]
+  | _                  => emsub
+  end.
+
+Coercion of_Bind : Bind >-> Env.
+
+Definition b2r b : Restr := 
+  match b with
+  | isEQ u v => u ≠ v
+  | isCONS u => NCONS u
+  end.
+Coercion b2r : Bind >-> Restr.
+
+Definition csubst (c : Cenv) (e : Bind) := 
+  let: (ce, r) := c in
+  (comp ce e, rsubst r e).
+
+Definition restr (c : Cenv) (b : Bind) := 
+  let: (e, r) := c in (e, b2r b :: r).
+
+Lemma substE (e1 e2 : Env) : 
+  (forall v : Var, v /s/ e1 = v /s/ e2) -> e1 = e2.
+Proof.
+by move=> E; apply/fsfunP=> [n]; move: (E n).
+Qed.
+
+Lemma substP (f : Exp -> Exp) (env : Env): 
+  (forall v : Var, env v = f v) ->
+  (forall a, f 'a = 'a) ->
+  (forall e1 e2, f (CONS e1 e2) = CONS (f e1) (f e2)) ->
+  (forall e, e /s/ env = f e).
+Proof.
+move=> ???; elim=> /= [[[]|?]|?->?->]//=.
+Qed.
+
+Lemma emsubv (v : Var): 
+  emsub v = v.
+Proof. by rewrite fsfun_dflt /= ?finsupp0 ?inE. Qed.
+
+Lemma comp_env x e1 e2: 
+  x /s/ (comp e1 e2) = (x /s/ e1) /s/ e2.
+Proof.
+rewrite -[(x /s/ e1) /s/ e2]/((fun y => (y /s/ e1) /s/ e2) x).
+apply/substP=> // ?.
+rewrite /comp fsfunE; case: ifP=> //= /negbT.
+by rewrite inE negb_or => /andP[??]; rewrite fsfun_dflt //= fsfun_dflt.
+Qed.
+
+Lemma comp0e e1: comp emsub e1 = e1.
+Proof. by apply/substE=> v; rewrite comp_env /= emsubv. Qed.
+
+Lemma compe0 e1: comp e1 emsub = e1.
+Proof. 
+apply/substE=> v. rewrite comp_env /= -{2}[e1 v]/(id (e1 v)).
+apply/substP=> //; exact/emsubv.
+Qed.
+
+Lemma compA e1 e2 e3 : comp e1 (comp e2 e3) = comp (comp e1 e2) e3.
+Proof. by apply/substE=> ?; rewrite ?comp_env. Qed.
+
+Lemma subst_var (v u : Var) (e : Exp): 
+  v /s/ ([fsfun emsub with u |-> e]) = if v == u then e else v.
+Proof. by rewrite /= fsfun_withE emsubv. Qed.
+
+Lemma subst_fv e (e1 e2 : Env): 
+  (forall x, x \in FVExp e -> e1 x = e2 x) ->
+  e /s/ e1 = e /s/ e2.
+Proof.
+elim: e=> /= [[[]|?]|? IHe1 ? IHe2 H]//; first by (apply; rewrite ?inE).
+by apply/congr2; rewrite (IHe1, IHe2) // => ? I; rewrite H // ?inE I ?orbT.
+Qed.
+
+Definition whole_env (e : Env)  := 
+  [fset x | a in finsupp e, x in FVExp (e a)].
+
+Lemma mem_whole_env x e: 
+  reflect (exists2 y, y \in finsupp e & (x \in FVExp (e y)))
+  (x \in whole_env e).
+Proof.
+apply/(iffP idP)=> [/imfset2P[y ? [? /[swap]<- ?]]|[y *]].
+- by exists y.
+apply/imfset2P; exists y=> //; by exists x.
+Qed.
+
+Definition whole_rs (rs : seq Restr) := 
+  [fset x | a in rs, x in FVRestr a].
+
+Lemma mem_whole_rs x rs: 
+  reflect (exists2 y, (y \in rs) & (x \in FVRestr y))
+  (x \in whole_rs rs).
+apply/(iffP idP)=> [/imfset2P[y ? [? /[swap]<- ?]]|[y *]].
+- by exists y.
+apply/imfset2P; exists y=> //; by exists x.
+Qed.
+
+Definition whole (e : Cenv) : {fset Var} :=
+  whole_env e.1 `|` whole_rs e.2.
+
+Lemma whole_env_substin (env : Env) v: 
+  v \in finsupp env ->
+  FVExp (env v) `<=` whole_env env.
+Proof. move=> ?; apply/fsubsetP=> ??; apply/mem_whole_env; by exists v. Qed.
+
+Lemma whole_env_subst (env : Env) (e : Exp): 
+  FVExp (e /s/ env) `<=` FVExp e `|` whole_env env.
+Proof.
+elim: e=> /= [[[]|v]|? IHe1 ? IHe2] //=.
+- case: (boolP (v \in finsupp env))=> [?|?].
+  apply/(fsubset_trans (whole_env_substin _ _ _))=> //.
+  by rewrite fsubsetUr.
+  by rewrite fsfun_dflt //= fsubsetUl.
+rewrite fsubUset; apply/andP; split.
+- apply/(fsubset_trans IHe1).
+  by rewrite [FVExp _ `|` FVExp _]fsetUC -fsetUA fsubsetUr.
+apply/(fsubset_trans IHe2); by rewrite -fsetUA fsubsetUr.
+Qed.
+
+
+Lemma whole_subst (env : Env) (rs : seq Restr) (e : Exp): 
+  FVExp (e /s/ env) `<=` FVExp e `|` whole (env, rs).
+Proof. by rewrite /whole fsetUA /= fsubsetU // whole_env_subst. Qed.
+
+Lemma whole_restr {e rs r}: 
+  whole (e, r :: rs) = FVRestr r `|` whole (e, rs).
+Proof.
+rewrite /whole /= fsetUC [whole_env _ `|` _]fsetUC fsetUA.
+apply/congr2=> //; apply/fsetP=> ?; rewrite inE.
+apply/(sameP idP)/(iffP idP)=> [/orP[]I|/mem_whole_rs[]].
+- apply/mem_whole_rs; exists r=> //=; by rewrite inE eq_refl.
+- case/mem_whole_rs: I=> y I *. apply/mem_whole_rs; exists y=> //.
+  by rewrite inE orbC I.
+move=> x; rewrite inE=> /orP[/eqP->-> //|??]; apply/orP; right.
+by apply/mem_whole_rs; exists x.
+Qed.
+
+Lemma whole_with {env : Env} {v : Var} {e : Exp} {rs}: 
+  whole ([fsfun env with v |-> e], rs) `<=` v |` (FVExp e) `|` whole (env, rs).
+Proof.
+rewrite -fsetUA fsubsetU //; apply/orP; right.
+rewrite /whole /= fsetUA fsetSU //.
+apply/fsubsetP=> ? /mem_whole_env[x].
+rewrite finsupp_with; case: ifP=> [/eqP->|].
+- rewrite fsfun_withE ?inE. case: ifP=> //= ???; apply/orP; right.
+  by apply/mem_whole_env; exists x.
+rewrite ?inE fsfun_withE; case: ifP=> //= [???->//|*]; apply/orP; right.
+by apply/mem_whole_env; exists x.
+Qed.
+
+Lemma comp_var (v : Var) env env': 
+  comp env env' v = (env v) /s/ env'.
+Proof. by rewrite -[comp env env' v]/(v /s/ (comp env env')) comp_env. Qed.
+
+
+Lemma whole_comp {env : Env} {v : Var} {e : Exp} {rs}: 
+  whole (comp env [fsfun emsub with v |-> e], rs) `<=` (FVExp e) `|` whole (env, rs).
+Proof.
+rewrite /whole /= fsetUA fsetSU //.
+apply/fsubsetP=> ? /mem_whole_env[x]; rewrite comp_var /comp.
+rewrite inE=> /(fsubsetP finsupp_fsfun); rewrite inE.
+case: (boolP (x \in finsupp env))=> /= [? _|?].
+- move/(fsubsetP (whole_env_subst _ _)); rewrite inE=> /orP[?|].
+  apply/orP; right; apply/mem_whole_env; by exists x.
+- case/mem_whole_env=> ?; rewrite finsupp_with; case: ifP=> [|?].
+  - by rewrite finsupp0 ?inE andbF.
+  by rewrite ?inE orbF=> /eqP->; rewrite fsfun_with=>->.
+rewrite finsupp_with; case: ifP; first by rewrite finsupp0 ?inE andbF.
+rewrite ?inE orbF fsfun_dflt // => ? /eqP-> /=.
+by rewrite fsfun_with=>->. 
+Qed.
+
+Lemma whole_cas {v a env rs}: 
+  whole (env, [seq cas v a i | i <- rs]) `<=`
+  FVArg a `|` whole (env, rs).
+Proof.
+rewrite /whole /= [FVArg _ `|` _]fsetUC -fsetUA fsetUS //.
+apply/fsubsetP=> x /mem_whole_rs[y /mapP[z]].
+rewrite /cas. case: z=> [r1 r2|].
+- case: ifP=> [/eqP->|].
+  - case: ifP=> [/eqP-> ? -> /=|]. 
+    - rewrite fsetUid inE=>->; by rewrite orbT.
+    move=> ?? -> /=; rewrite ?inE=> /orP[->|H]; first by rewrite orbT.
+    apply/orP; left; apply/mem_whole_rs; exists (v ≠ r2)=> //=.
+    by rewrite ?inE H orbT.
+  - case: ifP=> [/eqP-> ?? -> /=|].
+    - rewrite ?inE=> /orP[H|->]; last by rewrite orbT.
+    apply/orP; left; apply/mem_whole_rs; exists (r1 ≠ v)=> //=.
+    by rewrite ?inE H.
+  move=> ??? -> ?; rewrite ?inE.
+  apply/orP; left; apply/mem_whole_rs; by exists (r1 ≠ r2)=> //=.
+move=> u ? -> /= ?; rewrite ?inE.
+apply/orP; left; apply/mem_whole_rs; by exists (NCONS u)=> //=.
+Qed.
+
+Definition aux (e : Env) (f : {fset Var}): {fset Var} :=
+  [fset x | a in f, x in FVExp (e a)].
+
+Lemma mem_aux (e : Env) (f : {fset Var}) x: 
+  reflect (exists2 y, y \in f & x \in FVExp (e y))
+  (x \in aux e f).
+Proof.
+apply/(iffP idP)=> [/imfset2P[y ? [? /[swap]-> ?]]|[y ??]].
+- by exists y.
+apply/imfset2P; exists y=> //; by exists x.
+Qed.
+
+Lemma auxU f g e: aux e (f `|` g) = aux e f `|` aux e g.
+Proof.
+apply/fsetP=> ?; apply/(sameP idP)/(iffP idP); rewrite ?inE.
+- by case/orP=> /mem_aux[x I ?]; apply/mem_aux; exists x=> //; rewrite ?inE I ?orbT.
+case/mem_aux=> x.
+by rewrite ?inE=> /orP[] I ?; apply/orP; [left | right]; apply/mem_aux; exists x.
+Qed.
+
+Lemma aux_FVExp e a : aux e (FVExp a) = FVExp a /s/ e.
+Proof.
+elim: a=> [|? IH1 ? IH2] /=; last by rewrite auxU IH1 IH2.
+- case=> [[]?|v] //=; apply/fsetP=> ?; apply/(sameP idP)/(iffP idP).
+  - by rewrite inE.
+  - case/mem_aux=> ?; by rewrite inE.
+  - move=> ?; apply/mem_aux; exists v=> //; by rewrite ?inE.
+  by case/mem_aux=> ?; rewrite ?inE=> /eqP->.
+Qed.
+
+Lemma memNwhole k rs v env env'  e1 l: 
+  max_set (whole (env, rs)) <= k ->
+  v < l -> k < l ->
+  (env v) /s/ [fsfun env' with l |-> e1] = 
+  (env v) /s/ env'.
+Proof.
+move/mem_max_set=> m ??.
+case: (boolP (v \in finsupp env))=> [/whole_env_substin H|?].
+- have: forall x, x \in FVExp (env v) -> x <= k.
+  move=> ? /(fsubsetP H) I; apply/m; by rewrite inE /= I.
+  elim: (env v)=> [[[]|u /(_ _ (fset11 _))]|] //=.
+  - rewrite fsfun_withE; case: ifP; slia.
+  move=> ? IHe1 ? IHe2 I; rewrite IHe1 ?IHe2 //; 
+  by move=> ? I'; apply/I; rewrite ?inE I' ?orbT.
+rewrite fsfun_dflt //= fsfun_withE; case: ifP; slia.
+Qed.
+
+Lemma whole_cons rs (env : Env) (v : Var) e1 e2: 
+  env v = CONS e1 e2 -> 
+  ((FVExp e1 `<=` whole (env, rs)) * (FVExp e2 `<=` whole (env, rs)))%type.
+Proof.
+case: (boolP (v \in finsupp env))=> [/whole_env_substin|?].
+- move=> /[swap]-> /=; rewrite fsubUset /whole /= => /andP[H1 H2].
+  by rewrite ?fsubsetU // (H1, H2).
+by rewrite fsfun_dflt.
+Qed.
+
+Section ContradictTh.
+
+Lemma cont_isCONS rs v: contradict rs (isCONS v) = (NCONS v \in rs).
+Proof.
+elim: rs=> //= a ?; rewrite inE /contr; case: a=> // a ->; apply/orb_id2r=> ?.
+by apply/(sameP _ eqP)/(iffP eqP)=> [|[]]->.
+Qed.
+
+Lemma cont_isEQ rs v u: 
+  reflect (exists r1 r2, r1 ≠ r2 \in rs /\
+  ((r1, r2) = (v, u) \/ (r2, r1) = (v, u)))
+  (contradict rs (isEQ v u)).
+Proof. 
+apply/(iffP hasP)=> [[[]//= r1 r2 ?]|[r1 [r2 [?]]]] /pred2P ?.
+- by exists r1, r2.
+by exists (r1 ≠ r2).
+Qed.
+
+Lemma Ncont_isEQ rs v u: 
+  reflect (forall r1 r2, r1 ≠ r2 \in rs ->
+  ((r1, r2) <> (v, u) /\ (r2, r1) <> (v, u)))
+  (~~ (contradict rs (isEQ v u))).
+Proof.
+apply/(iffP hasPn)=> [H ?? /H|H []// ?? /H[/eqP/[swap]/eqP]]; rewrite negb_or.
+- by case/andP=>/eqP?/eqP.
+by move->=>->.
+Qed. 
+
+Lemma ncontr_cons e rs v: 
+  ncontr_env e (NCONS v :: rs) <->
+  (ncontr_env e rs /\ ncontr_ncons e v).
+Proof.
+split=> [][] H1 H2; do ?split.
+- by move=> ?? I; apply/H1; rewrite ?inE I orbT.
+- by move=> ? I; apply/H2; rewrite ?inE I orbT.
+- by apply/H2; rewrite ?inE eq_refl.
+- by move=> ??; rewrite inE=> /orP[]//; case: H1=> H ? /H.
+by move=> ?; rewrite inE=> /orP[/eqP[->]|]//; case: H1=> ? H /H.
+Qed.
+
+Lemma ncontr_eq e rs v u: 
+  ncontr_env e (v ≠ u :: rs) <->
+  (ncontr_env e rs /\ ncontr_neq e v u).
+Proof.
+split=> [][] H1 H2; do ?split.
+- by move=> ?? I; apply/H1; rewrite ?inE I orbT.
+- by move=> ? I; apply/H2; rewrite ?inE I orbT.
+- by apply/H1; rewrite ?inE eq_refl.
+- by move=> ??; rewrite inE=> /orP[/eqP[->->]|]//; case: H1=> H ? /H.
+by move=> ?; rewrite inE=> /orP[]//; case: H1=> ? H /H.
+Qed.
+
+Lemma ncontr_whole env' env v rs e: 
+  max_set (whole (env', rs)) < v ->
+  ncontr_env env rs ->
+  ncontr_env [fsfun env with v |-> e] rs.
+Proof.
+move/mem_max_set'=> H.
+have: {in whole_rs rs, forall x : nat, x < v}=> [? I|{H}H].
+- by apply/H; rewrite /whole /= ?inE I orbT.
+case=> H1 H2; split=> [r1 r2 I|].
+  - have: {subset FVRestr (r1 ≠ r2) <= whole_rs rs}.
+    move=> ??; apply/mem_whole_rs; by exists (r1 ≠ r2).
+  case: r1 r2 I=> [[? [[? /H1 //]|u /H1 N I]]|] /=.
+  - have ?: u < v.
+    - by apply/H/I=> /=; rewrite ?inE eq_refl.
+    move=> ? /= /[dup] ?; rewrite fsfun_withE; case: ifP; try slia.
+    move=> *; exact/N.
+  move=> u [[? /H1 N I]|] /=.
+    - have ?: u < v by apply/H/I=> /=; rewrite ?inE eq_refl.
+      move=> /[swap] ? /= /[dup] ?; rewrite fsfun_withE; case: ifP; try slia.
+    move=> *; exact/N.
+  move=> u' /H1 N I .
+  - have ?: u < v by apply/H/I=> /=; rewrite ?inE eq_refl.
+  - have ?: u' < v by apply/H/I=> /=; rewrite ?inE eq_refl orbT.
+  move=> /[dup] ? /[dup] ? /=; rewrite ?fsfun_withE; do ?case: ifP; try slia.
+  move=> *; exact/N.
+move=> [[]|] // u I.
+have: {subset FVRestr (NCONS u) <= whole_rs rs}.
+move=> ??; apply/mem_whole_rs; by exists (NCONS u).
+move: I=> /[swap] /= I /H2 N.
+- have ? : u < v by apply/H/I; rewrite ?inE eq_refl.
+rewrite /ncontr_ncons /= fsfun_withE; case: ifP; slia.
+Qed.
+
+Lemma fmap_of0 xs: mkEnv xs [::] = emsub.
+Proof. by case: xs. Qed.
+
+Lemma fmap_ofcons v vs x xs: mkEnv (x :: xs) (v :: vs) = 
+  [fsfun mkEnv xs vs with x |-> v].
+Proof. by []. Qed.
+
+Lemma whole_fmap {xs} {e : Env} {l rs}: 
+  whole (mkEnv xs (map (subst^~ e) l), rs) `<=` 
+  whole (e, rs) `|` [fset x | y in l, x in FVExp y].
+Proof.
+rewrite /whole /= [(_ `|` _)`|` _]fsetUC fsetUA fsetSU //.
+apply/fsubsetP=> y /mem_whole_env [x].
+elim: xs l=> [l|b l' IHxs [/=|a l /=]]. 
+- rewrite /mkEnv /= . case: l=> //=; by rewrite finsupp0.
+- by rewrite fmap_of0 /= finsupp0.
+rewrite fmap_ofcons fsfun_withE; case: ifP=> [??|E].
+- move/(fsubsetP (whole_env_subst _ _)); rewrite ?inE=> /orP[|->].
+  - move=> ?; apply/orP; left; apply/imfset2P; exists a.
+    - by rewrite /= mem_head.
+   by exists y.  
+  by rewrite orbT.
+have /fsubsetP/[apply]:  
+  finsupp [fsfun mkEnv l' [seq x0 /s/ e | x0 <- l] with b |-> a /s/ e] `<=`
+  b |` finsupp (mkEnv l' [seq x0 /s/ e | x0 <- l]).
+- rewrite finsupp_with; case: ifP=> // ?. 
+  exact/(fsubset_trans (fsubD1set _ _ ))/fsubsetU1.
+rewrite ?inE E /==> /IHxs /[apply]; rewrite ?inE => /orP[/imfset2P[z I [w ? ->]]|->].
+- apply/orP; left. apply/imfset2P; exists z; first by rewrite ?inE I orbT.
+  by exists w.
+by rewrite orbT.
+Qed.
+
+Lemma subst_closed e env: closed e -> e = e /s/ env.
+Proof.
+elim: e=> [[[]|? /eqP /= /(congr1 (fun x => #|` x|))]|? IH1 ? IH2] //=.
+- by rewrite cardfs1.
+rewrite /closed /= fsetU_eq0=> /andP[??].
+by apply/congr2; rewrite -(IH1, IH2).
+Qed.
+
+Lemma fmap_cat e1 e2 t:
+  (forall x, x \in e1 -> closed x) ->
+  size t = (size e1 + size e2)%N  ->
+  mkEnv t (e1 ++ e2) =
+  comp (mkEnv t e1) (mkEnv (drop (size e1) t) e2).
+Proof.
+elim: e1 t=> /= [?|?? IH [|?? c /=?]]; first by rewrite fmap_of0 comp0e drop0.
+- slia.
+rewrite ?fmap_ofcons; apply/substE=> v; rewrite comp_env /= ?fsfun_withE.
+case: ifP=> ?; first (rewrite -subst_closed //; exact/c/mem_head).
+rewrite IH ?comp_var // => [? I|]; last slia; apply/c; by rewrite ?inE I orbT.
+Qed.
+
+End ContradictTh.
+
+
+
+
+
