utilities.v
@@ -1,0 +1,179 @@
+From Coq Require Import Lia.
+From mathcomp Require Import ssreflect ssrnat eqtype ssrbool ssrfun seq.
+From mathcomp Require Import finmap fintype choice.
+
+Open Scope fmap_scope.
+Open Scope fset_scope.
+
+Ltac ssrnatify_rel :=
+ match goal with
+  (* less or equal (also codes for strict comparison in ssrnat) *)
+  | H : is_true (leq _ _) |- _ => move/leP: H => H
+  | H : context [ is_true (leq ?a ?b)] |- _ =>
+     rewrite <- (rwP (@leP a b)) in H
+  | |- is_true (leq _ _) => apply/leP
+  | |- context [ is_true (leq ?a ?b)] => rewrite <- (rwP (@leP a b))
+  (* Boolean equality *)
+  | H : is_true (@eq_op _ _ _) |- _ => move/eqP: H => H
+  | |- is_true (@eq_op _ _ _) => apply/eqP
+  | H : context [ is_true (@eq_op _ _ _)] |- _ =>
+     rewrite <-  (rwP (@eqP _ _ _)) in H
+  | |- context [ is_true (@eq_op _ ?x ?y)] => rewrite <- (rwP (@eqP _ x y))
+  (* Negated boolean equality *)
+  | H : is_true (negb (@eq_op _  _ _)) |- _ => move/eqP: H => H
+  | |- is_true (negb (@eq_op _  _ _)) => apply/eqP
+  | H : context [ is_true (negb (@eq_op _ _ _))] |- _ =>
+     rewrite <-  (rwP (@eqP _ _ _)) in H
+  | |- context [ is_true (negb (@eq_op _ ?x ?y))] =>
+     rewrite <- (rwP (@eqP _ x y))
+  | H : (negb (@eq_op _  _ _)) = true |- _ => move/eqP: H => H
+  | |- (negb (@eq_op _  _ _)) = true => apply/eqP
+  | H : context [ (negb (@eq_op _ _ _)) = true ] |- _ =>
+     rewrite <-  (rwP (@eqP _ _ _)) in H
+  | |- context [ (negb (@eq_op _ ?x ?y)) = true ] =>
+     rewrite <- (rwP (@eqP _ x y))
+
+  | H : (leq _ _) = true |- _ => move/leP: H => H
+  | H : context [ (leq ?a ?b) = true] |- _ =>
+     rewrite <- (rwP (@leP a b)) in H
+  | |- (leq _ _) = true => apply/leP
+  | |- context [(leq ?a ?b) = true] => rewrite <- (rwP (@leP a b))
+  (* Boolean equality *)
+  | H : (@eq_op _ _ _) = true |- _ => move/eqP: H => H
+  | |- (@eq_op _ _ _) = true => apply/eqP
+  | H : context [(@eq_op _ _ _) = true] |- _ =>
+     rewrite <-  (rwP (@eqP _ _ _)) in H
+  | |- context [(@eq_op _ ?x ?y) = true] => rewrite <- (rwP (@eqP _ x y))
+
+  (* Negated lt *)
+  | H : is_true (negb (leq (S _) _)) |- _ => move: H; rewrite -leqNgt=> H
+  | H : context [ is_true (negb (leq (S _) _))] |- _ =>
+     rewrite -leqNgt in H
+  | |- is_true (negb (leq (S _) _)) => rewrite -leqNgt
+  | |- context [ is_true (negb (leq (S _) _))] => rewrite -leqNgt
+
+  (* Negated leq *)
+  | H : is_true (negb (leq _ _)) |- _ => move: H; rewrite -ltnNge=> H
+  | H : context [ is_true (negb (leq _ _))] |- _ =>
+     rewrite -ltnNge in H
+  | |- is_true (negb (leq _ _)) => rewrite -ltnNge
+  | |- context [ is_true (negb (leq _ _))] => rewrite -ltnNge
+
+   (* = flase *)
+  | H : (_ = false) |- _ => move/negbT: H => H
+  | |- (_ = false) => apply/negP
+  | H : context [ (?a = false)] |- _ =>
+     rewrite <-  (rwP (@negP a)) in H
+  | |- context [ ?a = false] =>
+     rewrite <- (rwP (@negP a))
+
+ end.
+
+
+(* Converting ssrnat operation to their std lib analogues *)
+Ltac ssrnatify_op :=
+ match goal with
+  (* subn -> minus *)
+  | H : context [subn _ _] |- _ => rewrite -!minusE in H
+  | |- context [subn _ _] => rewrite -!minusE
+  (* addn -> plus *)
+  | H : context [addn _ _] |- _ => rewrite -!plusE in H
+  | |- context [addn _ _] => rewrite -!plusE
+  (* muln -> mult *)
+  | H : context [muln _ _] |- _ => rewrite -!multE in H
+  | |- context [muln _ _] => rewrite -!multE
+ end.
+
+(* Preparing a goal to be solved by lia by translating every formula *)
+(* in the context or the conclusion which expresses a constraint on *)
+(* some nat into the std lib, Prop, analogues *)
+Ltac ssrnatify :=
+  repeat progress ssrnatify_rel;
+  repeat progress ssrnatify_op.
+
+(* Preprocessing + lia *)
+Ltac slia := try (move=> * //=); do [ ssrnatify; lia | exfalso; ssrnatify; lia].
+
+Lemma foldr_monoid {T : Type} {f : T -> T -> T} {n s1 s2}: 
+associative f ->
+(forall x, f n x = x) ->
+(forall x, f x n = x) ->
+f (foldr f n s1) (foldr f n s2) =
+foldr f n (s1 ++ s2).
+Proof. by move=> A L R; elim: s1=> //= ??; rewrite -A=>->. Qed.
+
+Definition max_set (f : seq nat) : nat :=
+  foldr maxn 0 f.
+
+Lemma max_set0 : max_set fset0 = 0.
+Proof. by []. Qed.
+
+Lemma max_setin g x: 
+  x \in g -> x <= max_set g.
+Proof.
+elim: g=> //= a l IH; rewrite ?inE leq_max=> /orP[/eqP->|/IH->]; 
+by rewrite (leqnn, orbT).
+Qed.
+
+Lemma max_subset f g: {subset f <= g} -> max_set f <= max_set g.
+Proof.
+elim: f g=> //= a f IH g s; rewrite geq_max; apply/andP; split.
+- exact/max_setin/(s a)/mem_head.
+by apply/IH=> ? I; apply/s; rewrite inE I orbT.
+Qed.
+
+Lemma max_set_le {f h: {fset nat}} {k : nat}: 
+  max_set f <= k -> h `<=` f ->
+  max_set h <= k.
+Proof. move=> ? /fsubsetP /max_subset; slia.  Qed.
+
+Lemma max_add {f :{fset nat}} {k}: 
+  max_set f <= k -> max_set ([fset k.+1; k.+2] `|` f) <= k.+3.
+Proof.
+move=> ?. apply/(@leq_trans (max_set (k.+1 :: k.+2 :: f))).
+- apply/max_subset=> ?; by rewrite ?inE orbA.
+rewrite /= ?geq_max; apply/and3P; split; slia.
+Qed.
+
+Lemma max_setU f g: 
+  max_set (f `|` g) = maxn (max_set f) (max_set g).
+Proof.
+have->: maxn (max_set f) (max_set g) = max_set (f ++ g).
+exact/(foldr_monoid maxnA max0n maxn0).
+have /andP/anti_leq //: ((max_set (f `|` g) <= max_set (f ++ g)) /\ 
+      (max_set (f ++ g) <= max_set (f `|` g)))%type.
+split; apply/max_subset=> ?; by rewrite ?inE mem_cat.
+Qed.
+
+
+Lemma max_set_le2 {f g h : {fset nat}} {k}: 
+  max_set f <= k -> max_set g <= k -> h `<=` f `|` g ->
+  max_set h <= k.
+Proof.
+move=> s1 s2 ?.
+by apply/(@max_set_le (f `|` g))=> //; rewrite max_setU geq_max s1 s2.
+Qed.
+
+Lemma mem_max_set f k:
+  max_set f <= k -> {in f, forall x, x <= k}.
+Proof. move=> ?? /max_setin; slia. Qed.
+
+Lemma mem_max_set' f k:
+  max_set f < k -> {in f, forall x, x < k}.
+Proof. move=> ?? /max_setin; slia. Qed.
+
+Lemma fsfunE {K : choiceType} {V : eqType} S f y dflt: 
+  ([fsfun x in S => f x] : {fsfun K -> V for dflt}) y = 
+  if y \in S then f y else dflt y.
+Proof. 
+rewrite /fsfun_of_fun /fsfun_of_ffun Fsfun.of_ffunE.
+by case: insubP=> [[/=??->->]|/negbTE->].
+Qed.
+
+Lemma finsupp_fsfun {K : eqType} {V: choiceType} {f g : V -> K} {s : {fset V}}: 
+  finsupp ([fsfun x in s => f x] : {fsfun V -> K for g}) `<=` s.
+Proof.
+apply/fsubsetP=> ?; rewrite mem_finsupp fsfunE; case: ifP=> //.
+by rewrite eq_refl.
+Qed.
+
